LocallyNameless/STLC_funs.v
@@ -40,25 +40,17 @@ Inductive Tm : Type :=
 | annot      : Tm -> Ty -> Tm
 | unit       : Tm
 | elimUnit   : Tm -> Tm -> Tm
-| elimUnit'  : Tm -> Tm -> Tm
-| elimUnit'' : Tm
 | abort      : Tm -> Tm
 | pair       : Tm -> Tm -> Tm
 | outl       : Tm -> Tm
 | outr       : Tm -> Tm
 | elimProd   : Tm -> Tm -> Tm
-| elimProd'  : Tm -> Tm -> Tm
-| elimProd'' : Tm
 | inl        : Tm -> Tm
 | inr        : Tm -> Tm
 | case       : Tm -> Tm -> Tm -> Tm
-| case'      : Tm -> Tm -> Tm -> Tm
-| case''     : Tm
 | zero       : Tm
 | succ       : Tm -> Tm
-| rec        : Tm -> Tm -> Tm -> Tm
-| rec'       : Tm -> Tm -> Tm -> Tm
-| rec''      : Tm.
+| rec        : Tm -> Tm -> Tm -> Tm.
 
 Coercion fvar : Atom >-> Tm.
 Coercion bvar : nat >-> Tm.
@@ -95,35 +87,25 @@ Defined.
 
 #[export] Instance Open_Tm : Open nat Atom Tm :=
   fix open (t : Tm) (i : nat) (a : Atom) : Tm :=
-(*     let _ : Open nat Atom Tm := open in *)
     match t with
     | fvar a          => fvar a
     | bvar j          => if decide (i = j) then a else bvar j
-(*     | abs t'          => abs (t' {{ S i ~> a }}) *)
     | abs t'          => abs (open t' (S i) a)
     | app t1 t2       => app (open t1 i a) (open t2 i a)
     | annot t' A      => annot (open t' i a) A
     | unit            => unit
-    | elimUnit t1 t2  => elimUnit (open t1 i a) (open t2 (S i) a)
-    | elimUnit' t1 t2 => elimUnit' (open t1 i a) (open t2 i a)
-    | elimUnit''      => elimUnit''
+    | elimUnit t1 t2  => elimUnit (open t1 i a) (open t2 i a)
     | abort t'        => abort (open t' i a)
     | pair t1 t2      => pair (open t1 i a) (open t2 i a)
     | outl t'         => outl (open t' i a)
     | outr t'         => outr (open t' i a)
-    | elimProd t1 t2  => elimProd (open t1 i a) (open t2 (S (S i)) a)
-    | elimProd' t1 t2 => elimProd' (open t1 i a) (open t2 i a)
-    | elimProd''      => elimProd''
+    | elimProd t1 t2  => elimProd (open t1 i a) (open t2 i a)
     | inl t'          => inl (open t' i a)
     | inr t'          => inr (open t' i a)
-    | case t1 t2 t3   => case (open t1 i a) (open t2 (S i) a) (open t3 (S i) a)
-    | case' t1 t2 t3  => case' (open t1 i a) (open t2 i a) (open t3 i a)
-    | case''          => case''
+    | case t1 t2 t3   => case (open t1 i a) (open t2 i a) (open t3 i a)
     | zero            => zero
     | succ t'         => succ (open t' i a)
-    | rec t1 t2 t3    => rec (open t1 i a) (open t2 (S i) a) (open t3 i a)
-    | rec' t1 t2 t3   => rec' (open t1 i a) (open t2 i a) (open t3 i a)
-    | rec''           => rec''
+    | rec t1 t2 t3    => rec (open t1 i a) (open t2 i a) (open t3 i a)
     end.
 
 #[export] Instance Close_Tm : Close nat Atom Tm :=
@@ -135,26 +117,18 @@ Defined.
     | app t1 t2       => app (close t1 i a) (close t2 i a)
     | annot t' A      => annot (close t' i a) A
     | unit            => unit
-    | elimUnit t1 t2  => elimUnit (close t1 i a) (close t2 (S i) a)
-    | elimUnit' t1 t2 => elimUnit' (close t1 i a) (close t2 i a)
-    | elimUnit''      => elimUnit''
+    | elimUnit t1 t2  => elimUnit (close t1 i a) (close t2 i a)
     | abort t'        => abort (close t' i a)
     | pair t1 t2      => pair (close t1 i a) (close t2 i a)
     | outl t'         => outl (close t' i a)
     | outr t'         => outr (close t' i a)
-    | elimProd t1 t2  => elimProd (close t1 i a) (close t2 (S (S i)) a)
-    | elimProd' t1 t2 => elimProd' (close t1 i a) (close t2 i a)
-    | elimProd''      => elimProd''
+    | elimProd t1 t2  => elimProd (close t1 i a) (close t2 i a)
     | inl t'          => inl (close t' i a)
     | inr t'          => inr (close t' i a)
-    | case t1 t2 t3   => case (close t1 i a) (close t2 (S i) a) (close t3 (S i) a)
-    | case' t1 t2 t3  => case' (close t1 i a) (close t2 i a) (close t3 i a)
-    | case''          => case''
+    | case t1 t2 t3   => case (close t1 i a) (close t2 i a) (close t3 i a)
     | zero            => zero
     | succ t'         => succ (close t' i a)
-    | rec t1 t2 t3    => rec (close t1 i a) (close t2 (S i) a) (close t3 i a)
-    | rec' t1 t2 t3   => rec' (close t1 i a) (close t2 i a) (close t3 i a)
-    | rec''           => rec''
+    | rec t1 t2 t3    => rec (close t1 i a) (close t2 i a) (close t3 i a)
     end.
 
 #[export, refine] Instance OC_Tm :
@@ -184,25 +158,17 @@ match t with
 | annot t' A      => fv t'
 | unit            => []
 | elimUnit t1 t2  => fv t1 ++ fv t2
-| elimUnit' t1 t2 => fv t1 ++ fv t2
-| elimUnit''      => []
 | abort t'        => fv t'
 | pair t1 t2      => fv t1 ++ fv t2
 | outl t'         => fv t'
 | outr t'         => fv t'
 | elimProd t1 t2  => fv t1 ++ fv t2
-| elimProd' t1 t2 => fv t1 ++ fv t2
-| elimProd''      => []
 | inl t'          => fv t'
 | inr t'          => fv t'
 | case t1 t2 t3   => fv t1 ++ fv t2 ++ fv t3
-| case' t1 t2 t3  => fv t1 ++ fv t2 ++ fv t3
-| case''          => []
 | zero            => []
 | succ t'         => fv t'
 | rec t1 t2 t3    => fv t1 ++ fv t2 ++ fv t3
-| rec' t1 t2 t3   => fv t1 ++ fv t2 ++ fv t3
-| rec''           => []
 end.
 
 #[export, refine] Instance LocallyNameless_Tm :
@@ -275,16 +241,8 @@ Inductive LocallyClosed' : nat -> Tm -> Prop :=
 | LocallyClosed'_elimUnit :
   forall (i : nat) (t1 t2 : Tm),
     LocallyClosed' i t1 ->
-    LocallyClosed' (S i) t2 ->
-    LocallyClosed' i (elimUnit t1 t2)
-| LocallyClosed'_elimUnit' :
-  forall (i : nat) (t1 t2 : Tm),
-    LocallyClosed' i t1 ->
     LocallyClosed' i t2 ->
-    LocallyClosed' i (elimUnit' t1 t2)
-| LocallyClosed'_elimUnit'' :
-  forall (i : nat),
-    LocallyClosed' i elimUnit''
+    LocallyClosed' i (elimUnit t1 t2)
 | LocallyClosed'_abort :
   forall (i : nat) (t' : Tm),
     LocallyClosed' i t' -> LocallyClosed' i (abort t')
@@ -300,16 +258,8 @@ Inductive LocallyClosed' : nat -> Tm -> Prop :=
 | LocallyClosed'_elimProd :
   forall (i : nat) (t1 t2 : Tm),
     LocallyClosed' i t1 ->
-    LocallyClosed' (S (S i)) t2 ->
-    LocallyClosed' i (elimProd t1 t2)
-| LocallyClosed'_elimProd' :
-  forall (i : nat) (t1 t2 : Tm),
-    LocallyClosed' i t1 ->
     LocallyClosed' i t2 ->
-    LocallyClosed' i (elimProd' t1 t2)
-| LocallyClosed'_elimProd'' :
-  forall (i : nat),
-    LocallyClosed' i elimProd''
+    LocallyClosed' i (elimProd t1 t2)
 | LocallyClosed'_inl :
   forall (i : nat) (t' : Tm),
     LocallyClosed' i t' -> LocallyClosed' i (inl t')
@@ -319,18 +269,9 @@ Inductive LocallyClosed' : nat -> Tm -> Prop :=
 | LocallyClosed'_case :
   forall (i : nat) (t1 t2 t3 : Tm),
     LocallyClosed' i t1 ->
-    LocallyClosed' (S i) t2 ->
-    LocallyClosed' (S i) t3 ->
-    LocallyClosed' i (case t1 t2 t3)
-| LocallyClosed'_case' :
-  forall (i : nat) (t1 t2 t3 : Tm),
-    LocallyClosed' i t1 ->
     LocallyClosed' i t2 ->
     LocallyClosed' i t3 ->
-    LocallyClosed' i (case' t1 t2 t3)
-| LocallyClosed'_case'' :
-  forall (i : nat),
-    LocallyClosed' i case''
+    LocallyClosed' i (case t1 t2 t3)
 | LocallyClosed'_zero :
   forall (i : nat),
     LocallyClosed' i zero
@@ -340,18 +281,9 @@ Inductive LocallyClosed' : nat -> Tm -> Prop :=
 | LocallyClosed'_rec :
   forall (i : nat) (t1 t2 t3 : Tm),
     LocallyClosed' i t1 ->
-    LocallyClosed' (S i) t2 ->
-    LocallyClosed' i t3 ->
-    LocallyClosed' i (rec t1 t2 t3)
-| LocallyClosed'_rec' :
-  forall (i : nat) (t1 t2 t3 : Tm),
-    LocallyClosed' i t1 ->
     LocallyClosed' i t2 ->
     LocallyClosed' i t3 ->
-    LocallyClosed' i (rec' t1 t2 t3)
-| LocallyClosed'_rec'' :
-  forall (i : nat),
-    LocallyClosed' i rec''.
+    LocallyClosed' i (rec t1 t2 t3).
 
 #[export] Hint Constructors LocallyClosed' : core.
 
@@ -396,26 +328,18 @@ match t with
 | app t1 t2       => dec_LC_aux i t1 && dec_LC_aux i t2
 | annot t' A      => dec_LC_aux i t'
 | unit            => true
-| elimUnit t1 t2  => dec_LC_aux i t1 && dec_LC_aux (S i) t2
-| elimUnit' t1 t2 => dec_LC_aux i t1 && dec_LC_aux i t2
-| elimUnit''      => true
+| elimUnit t1 t2  => dec_LC_aux i t1 && dec_LC_aux i t2
 | abort t'        => dec_LC_aux i t'
 | pair t1 t2      => dec_LC_aux i t1 && dec_LC_aux i t2
 | outl t'         => dec_LC_aux i t'
 | outr t'         => dec_LC_aux i t'
-| elimProd t1 t2  => dec_LC_aux i t1 && dec_LC_aux (S (S i)) t2
-| elimProd' t1 t2 => dec_LC_aux i t1 && dec_LC_aux i t2
-| elimProd''      => true
+| elimProd t1 t2  => dec_LC_aux i t1 && dec_LC_aux i t2
 | inl t'          => dec_LC_aux i t'
 | inr t'          => dec_LC_aux i t'
-| case t1 t2 t3   => dec_LC_aux i t1 && dec_LC_aux (S i) t2 && dec_LC_aux (S i) t3
-| case' t1 t2 t3  => dec_LC_aux i t1 && dec_LC_aux i t2 && dec_LC_aux i t3
-| case''          => true
+| case t1 t2 t3   => dec_LC_aux i t1 && dec_LC_aux i t2 && dec_LC_aux i t3
 | zero            => true
 | succ t'         => dec_LC_aux i t'
-| rec t1 t2 t3    => dec_LC_aux i t1 && dec_LC_aux (S i) t2 && dec_LC_aux i t3
-| rec' t1 t2 t3   => dec_LC_aux i t1 && dec_LC_aux i t2 && dec_LC_aux i t3
-| rec''           => true
+| rec t1 t2 t3    => dec_LC_aux i t1 && dec_LC_aux i t2 && dec_LC_aux i t3
 end.
 
 #[export, refine] Instance Decidable_LocallyClosed' :
@@ -459,25 +383,17 @@ match t with
 | annot t' A      => annot (subst t' x u) A
 | unit            => unit
 | elimUnit t1 t2  => elimUnit (subst t1 x u) (subst t2 x u)
-| elimUnit' t1 t2 => elimUnit' (subst t1 x u) (subst t2 x u)
-| elimUnit''      => elimUnit''
 | abort t'        => abort (subst t' x u)
 | pair t1 t2      => pair (subst t1 x u) (subst t2 x u)
 | outl t'         => outl (subst t' x u)
 | outr t'         => outr (subst t' x u)
 | elimProd t1 t2  => elimProd (subst t1 x u) (subst t2 x u)
-| elimProd' t1 t2 => elimProd' (subst t1 x u) (subst t2 x u)
-| elimProd''      => elimProd''
 | inl t'          => inl (subst t' x u)
 | inr t'          => inr (subst t' x u)
 | case t1 t2 t3   => case (subst t1 x u) (subst t2 x u) (subst t3 x u)
-| case' t1 t2 t3  => case' (subst t1 x u) (subst t2 x u) (subst t3 x u)
-| case''          => case''
 | zero            => zero
 | succ t'         => succ (subst t' x u)
 | rec t1 t2 t3    => rec (subst t1 x u) (subst t2 x u) (subst t3 x u)
-| rec' t1 t2 t3   => rec' (subst t1 x u) (subst t2 x u) (subst t3 x u)
-| rec''           => rec''
 end.
 
 Notation "t [[ x := u ]]" := (subst t x u) (at level 69, left associativity).
@@ -513,26 +429,18 @@ match t with
 | app t1 t2       => app (open' t1 i u) (open' t2 i u)
 | annot t' A      => annot (open' t' i u) A
 | unit            => unit
-| elimUnit t1 t2  => elimUnit (open' t1 i u) (open' t2 (S i) u)
-| elimUnit' t1 t2 => elimUnit' (open' t1 i u) (open' t2 i u)
-| elimUnit''      => elimUnit''
+| elimUnit t1 t2  => elimUnit (open' t1 i u) (open' t2 i u)
 | abort t'        => abort (open' t' i u)
 | pair t1 t2      => pair (open' t1 i u) (open' t2 i u)
 | outl t'         => outl (open' t' i u)
 | outr t'         => outr (open' t' i u)
-| elimProd t1 t2  => elimProd (open' t1 i u) (open' t2 (S (S i)) u)
-| elimProd' t1 t2 => elimProd' (open' t1 i u) (open' t2 i u)
-| elimProd''      => elimProd''
+| elimProd t1 t2  => elimProd (open' t1 i u) (open' t2 i u)
 | inl t'          => inl (open' t' i u)
 | inr t'          => inr (open' t' i u)
-| case t1 t2 t3   => case (open' t1 i u) (open' t2 (S i) u) (open' t3 (S i) u)
-| case' t1 t2 t3  => case' (open' t1 i u) (open' t2 i u) (open' t3 i u)
-| case''          => case''
+| case t1 t2 t3   => case (open' t1 i u) (open' t2 i u) (open' t3 i u)
 | zero            => zero
 | succ t'         => succ (open' t' i u)
-| rec t1 t2 t3    => rec (open' t1 i u) (open' t2 (S i) u) (open' t3 i u)
-| rec' t1 t2 t3   => rec' (open' t1 i u) (open' t2 i u) (open' t3 i u)
-| rec''           => rec''
+| rec t1 t2 t3    => rec (open' t1 i u) (open' t2 i u) (open' t3 i u)
 end.
 
 Notation "t {[ i ~> u ]}" := (open' t i u) (at level 69, left associativity).
@@ -572,16 +480,6 @@ Qed.
 
 (** ** Local closure *)
 
-(*
-Definition cof (P : Atom -> Prop) : Prop :=
-  exists l : list Atom, forall x : Atom, x # l -> P x.
-*)
-
-(*
-Notation "'cof' x , P" :=
-  (exists l : list Atom, forall x : Atom, x # l -> P) (at level 100) : type_scope.
-*)
-
 Inductive lc : Tm -> Prop :=
 | lc_fvar :
   forall x : Atom,
@@ -590,18 +488,6 @@ Inductive lc : Tm -> Prop :=
   forall (t' : Tm) (l : list Atom)
     (Hlc' : forall x : Atom, x # l -> lc (t' {{ 0 ~> x }})),
     lc (abs t')
-(*
-| lc_abs :
-  forall (t' : Tm)
-    (Hlc' : exists l : list Atom, forall x : Atom, x # l -> lc (t' {{ 0 ~> x }})),
-    lc (abs t')
-*)
-(*
-| lc_abs :
-  forall (t' : Tm)
-    (Hlc' : cof x, lc (t' {{ 0 ~> x }})),
-    lc (abs t')
-*)
 | lc_app :
   forall (t1 t2 : Tm)
     (Hlc1 : lc t1)
@@ -613,16 +499,10 @@ Inductive lc : Tm -> Prop :=
     lc (annot t' A)
 | lc_unit : lc unit
 | lc_elimUnit :
-  forall (t1 t2 : Tm) (l : list Atom)
-    (Hlc1 : lc t1)
-    (Hlc2 : forall x : Atom, x # l -> lc (t2 {{ 0 ~> x }})),
-    lc (elimUnit t1 t2)
-| lc_elimUnit' :
   forall (t1 t2 : Tm)
     (Hlc1 : lc t1)
     (Hlc2 : lc t2),
-    lc (elimUnit' t1 t2)
-| lc_elimUnit'' : lc elimUnit''
+    lc (elimUnit t1 t2)
 | lc_abort :
   forall (t' : Tm)
     (Hlc' : lc t'),
@@ -641,16 +521,10 @@ Inductive lc : Tm -> Prop :=
     (Hlc' : lc t'),
     lc (outr t')
 | lc_elimProd :
-  forall (t1 t2 : Tm) (l : list Atom)
-    (Hlc1 : lc t1)
-    (Hlc2 : forall x y : Atom, x # l -> y # x :: l -> lc (t2 {{ 0 ~> x }} {{ 1 ~> y }})),
-    lc (elimProd t1 t2)
-| lc_elimProd' :
   forall (t1 t2 : Tm)
     (Hlc1 : lc t1)
     (Hlc2 : lc t2),
-    lc (elimProd' t1 t2)
-| lc_elimProd'' : lc elimProd''
+    lc (elimProd t1 t2)
 | lc_inl :
   forall (t' : Tm)
     (Hlc' : lc t'),
@@ -660,36 +534,22 @@ Inductive lc : Tm -> Prop :=
     (Hlc' : lc t'),
     lc (inr t')
 | lc_case :
-  forall (t1 t2 t3 : Tm) (l : list Atom)
-    (Hlc1 : lc t1)
-    (Hlc2 : forall x : Atom, x # l -> lc (t2 {{ 0 ~> x }}))
-    (Hlc3 : forall y : Atom, y # l -> lc (t3 {{ 0 ~> y }})),
-    lc (case t1 t2 t3)
-| lc_case' :
   forall (t1 t2 t3 : Tm)
     (Hlc1 : lc t1)
     (Hlc2 : lc t2)
     (Hlc3 : lc t3),
-    lc (case' t1 t2 t3)
-| lc_case'' : lc case''
+    lc (case t1 t2 t3)
 | lc_zero : lc zero
 | lc_succ :
   forall (t' : Tm)
     (Hlc' : lc t'),
     lc (succ t')
 | lc_rec :
-  forall (t1 t2 t3 : Tm) (l : list Atom)
-    (Hlc1 : lc t1)
-    (Hlc2 : forall x : Atom, x # l -> lc (t2 {{ 0 ~> x }}))
-    (Hlc3 : lc t3),
-    lc (rec t1 t2 t3)
-| lc_rec' :
   forall (t1 t2 t3 : Tm)
     (Hlc1 : lc t1)
     (Hlc2 : lc t2)
     (Hlc3 : lc t3),
-    lc (rec' t1 t2 t3)
-| lc_rec'' : lc rec''.
+    lc (rec t1 t2 t3).
 
 #[export] Hint Constructors lc : core.
 
@@ -702,7 +562,6 @@ Proof.
     rewrite 1?IHHlc, 1?IHHlc1, 1?IHHlc2, 1?IHHlc3; f_equal;
     try now auto;
     try now eapply (open_open _ 0 (S j)); auto.
-  now eapply open_open, open_open, H; auto.
 Qed.
 
 Lemma open_lc :
@@ -749,14 +608,6 @@ Proof.
   induction Ht; cbn; intros; try now auto.
   - apply lc_abs with (x :: l).
     now intros y Hy; rewrite subst_open; auto.
-  - apply lc_elimUnit with (x :: l); [now apply IHHt |].
-    now intros y Hy; rewrite subst_open; auto.
-  - apply lc_elimProd with (x :: l); [now apply IHHt |];
-     intros y z Hy Hz; rewrite !subst_open; auto.
-  - apply lc_case with (x :: l); [now apply IHHt | |];
-      intros y Hy; rewrite subst_open; auto.
-  - now apply lc_rec with (x :: l); [now apply IHHt1 | | now apply IHHt2];
-      intros y Hy; rewrite subst_open; auto.
 Qed.
 
 Lemma lc_open' :
@@ -829,25 +680,17 @@ match t with
 | annot t' A      => 1 + size t'
 | unit            => 1
 | elimUnit t1 t2  => 1 + size t1 + size t2
-| elimUnit' t1 t2 => 1 + size t1 + size t2
-| elimUnit''      => 1
 | abort t'        => 1 + size t'
 | pair t1 t2      => 1 + size t1 + size t2
 | outl t'         => 1 + size t'
 | outr t'         => 1 + size t'
 | elimProd t1 t2  => 1 + size t1 + size t2
-| elimProd' t1 t2 => 1 + size t1 + size t2
-| elimProd''      => 1
 | inl t'          => 1 + size t'
 | inr t'          => 1 + size t'
 | case t1 t2 t3   => 1 + size t1 + size t2 + size t3
-| case' t1 t2 t3  => 1 + size t1 + size t2 + size t3
-| case''          => 1
 | zero            => 1
 | succ t'         => 1 + size t'
 | rec t1 t2 t3    => 1 + size t1 + size t2 + size t3
-| rec' t1 t2 t3   => 1 + size t1 + size t2 + size t3
-| rec''           => 1
 end.
 
 Lemma size_open :
@@ -866,26 +709,18 @@ match t with
 | app t1 t2       => decide_lc' a t1 && decide_lc' a t2
 | annot t' A      => decide_lc' a t'
 | unit            => true
-| elimUnit t1 t2  => decide_lc' a t1 && decide_lc' a (t2 {{ 0 ~> a }})
-| elimUnit' t1 t2 => decide_lc' a t1 && decide_lc' a t2
-| elimUnit''      => true
+| elimUnit t1 t2  => decide_lc' a t1 && decide_lc' a t2
 | abort t'        => decide_lc' a t'
 | pair t1 t2      => decide_lc' a t1 && decide_lc' a t2
 | outl t'         => decide_lc' a t'
 | outr t'         => decide_lc' a t'
-| elimProd t1 t2  => decide_lc' a t1 && decide_lc' a (t2 {{ 0 ~> a }} {{ 1 ~> a }})
-| elimProd' t1 t2 => decide_lc' a t1 && decide_lc' a t2
-| elimProd''      => true
+| elimProd t1 t2  => decide_lc' a t1 && decide_lc' a t2
 | inl t'          => decide_lc' a t'
 | inr t'          => decide_lc' a t'
-| case t1 t2 t3   => decide_lc' a t1 && decide_lc' a (t2 {{ 0 ~> a }}) && decide_lc' a (t3 {{ 0 ~> a }})
-| case' t1 t2 t3  => decide_lc' a t1 && decide_lc' a t2 && decide_lc' a t3
-| case''          => true
+| case t1 t2 t3   => decide_lc' a t1 && decide_lc' a t2 && decide_lc' a t3
 | zero            => true
 | succ t'         => decide_lc' a t'
-| rec t1 t2 t3    => decide_lc' a t1 && decide_lc' a (t2 {{ 0 ~> a }}) && decide_lc' a t3
-| rec' t1 t2 t3   => decide_lc' a t1 && decide_lc' a t2 && decide_lc' a t3
-| rec''           => true
+| rec t1 t2 t3    => decide_lc' a t1 && decide_lc' a t2 && decide_lc' a t3
 end.
 (*
 Proof.
@@ -902,11 +737,6 @@ Proof.
     inversion Hlc; subst; try now eauto.
   - apply lc_abs with l; intros z Hz.
     admit.
-  - apply lc_elimUnit with l; [now eauto |].
-    intros z Hz.
-    apply lc_open.
-    apply IHt2 with x.
-    replace (t2 {{ S i ~> x }}) with (t2 {{ S i ~> x }} {{ 0 ~> z }}).
 Admitted.
 
 Lemma lc_open_invariant' :
@@ -926,36 +756,10 @@ Proof.
   functional induction (decide_lc' a t);
     try (now try destruct IHb; try destruct IHb0; try destruct IHb1;
       cbn; constructor; [auto | inversion 1..]).
-  - destruct IHb; constructor; [now eauto |].
-    inversion 1.
-    now specialize (Hlc' (fresh l) (fresh_spec l)); eauto.
-  - destruct IHb, IHb0; cbn; constructor; [now eauto | inversion 1..].
-    + now specialize (Hlc2 (fresh l0) (fresh_spec l0)); eauto.
-    + now specialize (Hlc2 (fresh l0) (fresh_spec l0)); eauto.
-    + now specialize (Hlc2 (fresh l) (fresh_spec l)); eauto.
-  - destruct IHb, IHb0; cbn; constructor; [| inversion 1..].
-    + apply lc_elimProd with []; [easy |].
-      intros x y _ Hy.
-      admit.
-    + specialize (Hlc2 (fresh l0) (fresh (fresh l0 :: l0)) ltac:(auto) ltac:(auto)).
-      eapply lc_open_invariant in Hlc2.
-      admit.
-    + admit.
-    + admit.
-  - destruct IHb; cbn; [| now constructor; inversion 1; eauto].
-    destruct IHb0; cbn; cycle 1.
-    + constructor; inversion 1.
-      now eapply n, lc_open_invariant, Hlc2, fresh_spec.
-    + destruct IHb1; cbn; [now constructor; eauto |].
-      constructor; inversion 1; subst.
-      now eapply n, lc_open_invariant, Hlc3, fresh_spec.
-  - destruct IHb; cbn; [| now constructor; inversion 1; eauto].
-    destruct IHb0; cbn; cycle 1.
-    + constructor; inversion 1.
-      now eapply n, lc_open_invariant, Hlc2, fresh_spec.
-    + destruct IHb1; cbn; [now constructor; eauto |].
-      now constructor; inversion 1; eauto.
-Abort.
+  destruct IHb; constructor; [now apply lc_abs with [];  eauto |].
+  inversion 1.
+  now specialize (Hlc' (fresh l) (fresh_spec l)); eauto.
+Qed.
 
 #[export, refine] Instance Decidable_lc :
   forall t : Tm, Decidable (lc t) :=
@@ -965,7 +769,6 @@ Abort.
 }.
 Proof.
   split.
-  - induction t; cbn; try easy.
 Abort.
 
 (** * Contexts *)
@@ -1060,19 +863,10 @@ Inductive Typing : Ctx -> Tm -> Ty -> Prop :=
     (Hwf : WfCtx Γ),
     Typing Γ unit TyUnit
 | Typing_elimUnit :
-  forall (Γ : Ctx) (t1 t2 : Tm) (A : Ty) (l : list Atom)
-    (Ht1 : Typing Γ t1 TyUnit)
-    (Ht2 : forall x : Atom, x # l -> Typing ((x, TyUnit) :: Γ) (t2 {{ 0 ~> x }}) A),
-    Typing Γ (elimUnit t1 t2) A
-| Typing_elimUnit' :
   forall (Γ : Ctx) (t1 t2 : Tm) (A : Ty)
     (Ht1 : Typing Γ t1 TyUnit)
     (Ht2 : Typing Γ t2 (TyFun TyUnit A)),
-    Typing Γ (elimUnit' t1 t2) A
-| Typing_elimUnit'' :
-  forall (Γ : Ctx) (A : Ty)
-    (Hwf : WfCtx Γ),
-    Typing Γ elimUnit'' (TyFun (TyFun TyUnit A) (TyFun TyUnit A))
+    Typing Γ (elimUnit t1 t2) A
 | Typing_abort :
   forall (Γ : Ctx) (t' : Tm) (A : Ty)
     (Ht' : Typing Γ t' TyEmpty),
@@ -1092,19 +886,9 @@ Inductive Typing : Ctx -> Tm -> Ty -> Prop :=
     Typing Γ (outr t') B
 | Typing_elimProd :
   forall (Γ : Ctx) (t1 t2 : Tm) (A B C : Ty) (l : list Atom)
-    (Ht1 : Typing Γ t1 (TyProd A B))
-    (Ht2 : forall x y : Atom, x # l -> y # x :: l ->
-      Typing ((y, B) :: (x, A) :: Γ) (t2 {{ 0 ~> x }} {{ 1 ~> y }}) C),
-    Typing Γ (elimProd t1 t2) C
-| Typing_elimProd' :
-  forall (Γ : Ctx) (t1 t2 : Tm) (A B C : Ty) (l : list Atom)
     (Ht1 : Typing Γ t1 (TyFun A (TyFun B C)))
     (Ht2 : Typing Γ t2 (TyProd A B)),
-    Typing Γ (elimProd' t1 t2) C
-| Typing_elimProd'' :
-  forall (Γ : Ctx) (A B C : Ty)
-    (Hwf : WfCtx Γ),
-    Typing Γ elimProd'' (TyFun (TyFun A (TyFun B C)) (TyFun (TyProd A B) C))
+    Typing Γ (elimProd t1 t2) C
 | Typing_inl :
   forall (Γ : Ctx) (t' : Tm) (A B : Ty)
     (Ht' : Typing Γ t' A),
@@ -1114,21 +898,11 @@ Inductive Typing : Ctx -> Tm -> Ty -> Prop :=
     (Ht' : Typing Γ t' B),
     Typing Γ (inr t') (TySum A B)
 | Typing_case :
-  forall (Γ : Ctx) (t1 t2 t3 : Tm) (A B C : Ty) (l : list Atom)
-    (Ht1 : Typing Γ t1 (TySum A B))
-    (Ht2 : forall x : Atom, x # l -> Typing ((x, A) :: Γ) (t2 {{ 0 ~> x }}) C)
-    (Ht3 : forall y : Atom, y # l -> Typing ((y, B) :: Γ) (t3 {{ 0 ~> y }}) C),
-    Typing Γ (case t1 t2 t3) C
-| Typing_case' :
   forall (Γ : Ctx) (t1 t2 t3 : Tm) (A B C : Ty)
     (Ht1 : Typing Γ t1 (TyFun A C))
     (Ht2 : Typing Γ t2 (TyFun B C))
     (Ht3 : Typing Γ t3 (TySum A B)),
-    Typing Γ (case' t1 t2 t3) C
-| Typing_case'' :
-  forall (Γ : Ctx) (A B C : Ty)
-    (Hwf : WfCtx Γ),
-    Typing Γ case'' (TyFun (TyFun A C) (TyFun (TyFun B C) (TyFun (TySum A B) C)))
+    Typing Γ (case t1 t2 t3) C
 | Typing_zero :
   forall (Γ : Ctx)
     (Hwf : WfCtx Γ),
@@ -1138,17 +912,11 @@ Inductive Typing : Ctx -> Tm -> Ty -> Prop :=
     (Ht' : Typing Γ t' TyNat),
     Typing Γ (succ t') TyNat
 | Typing_rec :
-  forall (Γ : Ctx) (t1 t2 t3 : Tm) (A : Ty) (l : list Atom)
-    (Ht1 : Typing Γ t1 A)
-    (Ht2 : forall x : Atom, x # l -> Typing ((x, A) :: Γ) (t2 {{ 0 ~> x }}) A)
-    (Ht3 : Typing Γ t3 TyNat),
-    Typing Γ (rec t1 t2 t3) A
-| Typing_rec' :
   forall (Γ : Ctx) (t1 t2 t3 : Tm) (A : Ty)
     (Ht1 : Typing Γ t1 A)
     (Ht2 : Typing Γ t2 (TyFun A A))
     (Ht3 : Typing Γ t3 TyNat),
-    Typing Γ (rec' t1 t2 t3) A.
+    Typing Γ (rec t1 t2 t3) A.
 
 #[export] Hint Constructors Typing : core.
 
@@ -1189,25 +957,12 @@ Proof.
   intros * Ht.
   remember (Γ1 ++ Γ2) as G.
   revert Γ1 Γ2 Δ HeqG.
-  Time induction Ht; intros; subst; try now eauto.
+  induction Ht; intros; subst; try now eauto.
   - constructor; [easy |].
     unfold Binds in *.
     rewrite !in_app_iff; rewrite in_app_iff in HB.
     now firstorder.
   - apply Typing_abs with (l ++ map fst Γ1 ++ map fst Δ ++ map fst Γ2).
-    now intros; rewrite !app_comm_cons; apply H; cbn; auto.
-  - apply Typing_elimUnit with (l ++ map fst Γ1 ++ map fst Δ ++ map fst Γ2);
-      [now apply IHHt |].
-    now intros; rewrite !app_comm_cons; apply H; cbn; auto.
-  - apply Typing_elimProd with A B (l ++ map fst Γ1 ++ map fst Δ ++ map fst Γ2);
-      [now apply IHHt |].
-    now intros; rewrite !app_comm_cons; apply H; cbn; auto.
-  - apply Typing_case with A B (l ++ map fst Γ1 ++ map fst Δ ++ map fst Γ2);
-      [now apply IHHt | |].
-    + now intros; rewrite !app_comm_cons; apply H; cbn; auto.
-    + now intros; rewrite !app_comm_cons; apply H0; cbn; auto.
-  - apply Typing_rec with (l ++ map fst Γ1 ++ map fst Δ ++ map fst Γ2);
-      [now apply IHHt1 | | now apply IHHt2].
     now intros; rewrite !app_comm_cons; apply H; cbn; auto.
 Qed.
 
@@ -1240,27 +995,13 @@ Proof.
   intros * Ht Hu.
   remember (Δ ++ (x, A) :: Γ) as G.
   revert Δ x A Γ HeqG Hu.
-  Time induction Ht; cbn; intros; subst; try now eauto.
+  induction Ht; cbn; intros; subst; try now eauto.
   - apply WfCtx_app_cons in Hwf as Hwf'.
     decide_all.
     + apply Binds_inv' in HB as ->; [| easy].
       now apply weakening.
     + now apply Binds_app_cons_inv in HB as [ [-> ->] |]; auto.
   - apply Typing_abs with (x :: l).
-    intros y Hy; rewrite subst_open, !app_comm_cons by eauto.
-    now eapply H; cbn; auto.
-  - apply Typing_elimUnit with (x :: l); [now eapply IHHt |].
-    intros y Hy; rewrite subst_open, !app_comm_cons by eauto.
-    now eapply H; cbn; auto.
-  - apply Typing_elimProd with A B (x :: l); [now eapply IHHt |].
-    intros y z Hy Hz; rewrite 2!subst_open, 2!app_comm_cons by eauto.
-    now eapply H; cbn; auto.
-  - apply Typing_case with A B (x :: l); [now eapply IHHt | |].
-    + intros y Hy; rewrite subst_open, !app_comm_cons by eauto.
-      now eapply H; cbn; auto.
-    + intros y Hy; rewrite subst_open, !app_comm_cons by eauto.
-      now eapply H0; cbn; auto.
-  - apply Typing_rec with (x :: l); [now eapply IHHt1 | | now eapply IHHt2].
     intros y Hy; rewrite subst_open, !app_comm_cons by eauto.
     now eapply H; cbn; auto.
 Qed.
@@ -1317,11 +1058,6 @@ Inductive CbvValue : Tm -> Prop :=
     (Hlc' : forall x : Atom, x # l -> lc (t' {{ 0 ~> x }})),
     CbvValue (abs t')
 | CbvValue_unit : CbvValue unit
-| CbvValue_elimUnit'' : CbvValue elimUnit''
-| CbvValue_elimUnit''1 :
-  forall (t' : Tm)
-    (Hlc' : lc t'),
-    CbvValue (app elimUnit'' t')
 | CbvValue_abort :
   forall (t' : Tm)
     (Hlc' : lc t'),
@@ -1331,11 +1067,6 @@ Inductive CbvValue : Tm -> Prop :=
     CbvValue t1 ->
     CbvValue t2 ->
     CbvValue (pair t1 t2)
-| CbvValue_elimProd'' : CbvValue elimProd''
-| CbvValue_elimProd''1 :
-  forall (t1 : Tm)
-    (Hlc1 : lc t1),
-    CbvValue (app elimProd'' t1)
 | CbvValue_inl :
   forall v : Tm,
     CbvValue v ->
@@ -1344,31 +1075,11 @@ Inductive CbvValue : Tm -> Prop :=
   forall v : Tm,
     CbvValue v ->
     CbvValue (inr v)
-| CbvValue_case'' : CbvValue case''
-| CbvValue_case''1 :
-  forall (t1 : Tm)
-    (Hlc1 : lc t1),
-    CbvValue (app case'' t1)
-| CbvValue_case''2 :
-  forall (t1 t2 : Tm)
-    (Hlc1 : lc t1)
-    (Hlc2 : lc t2),
-    CbvValue (app (app case'' t1) t2)
 | CbvValue_zero : CbvValue zero
 | CbvValue_succ :
   forall (t' : Tm)
     (Hv' : CbvValue t'),
-    CbvValue (succ t')
-| CbvValue_rec'' : CbvValue rec''
-| CbvValue_rec''1 :
-  forall (t1 : Tm)
-    (Hlc1 : lc t1),
-    CbvValue (app rec'' t1)
-| CbvValue_rec''2 :
-  forall (t1 t2 : Tm)
-    (Hlc1 : lc t1)
-    (Hlc2 : lc t2),
-    CbvValue (app (app rec'' t1) t2).
+    CbvValue (succ t').
 
 #[export] Hint Constructors CbvValue : core.
 
@@ -1385,14 +1096,10 @@ Fixpoint cbvValue (t : Tm) : bool :=
 match t with
 | abs t'               => true
 | unit                 => true
-| elimUnit''           => true
 | abort t'             => true
 | pair t1 t2           => cbvValue t1 && cbvValue t2
 | inl t'               => cbvValue t'
 | inr t'               => cbvValue t'
-| case''               => true
-| app case'' _         => true
-| app (app case'' _) _ => true
 | zero                 => true
 | succ t'              => cbvValue t'
 | _                    => false
@@ -1407,12 +1114,6 @@ Proof.
   split.
   - induction t; inversion 1; auto.
     + admit.
-    + destruct t1; try easy.
-      * destruct t1_1; try easy.
-        constructor; admit.
-      * constructor; admit.
-    + constructor. admit.
-    + apply andb_prop in H1 as [H1 H2].
 Abort.
 
 (** *** Contraction *)
@@ -1428,17 +1129,9 @@ Inductive CbvContraction : Tm -> Tm -> Prop :=
     (Hlc : lc t),
     CbvContraction (annot t A) t
 | CbvContraction_elimUnit_unit :
-  forall (t : Tm) (l : list Atom)
-    (Hlc : forall x : Atom, x # l -> lc (t {{0 ~> x}})),
-    CbvContraction (elimUnit unit t) (t {[ 0 ~> unit ]})
-| CbvContraction_elimUnit'_unit :
   forall (t : Tm)
     (Hlc : lc t),
-    CbvContraction (elimUnit' unit t) (app t unit)
-| CbvContraction_elimUnit''_unit :
-  forall (t : Tm)
-    (Hlc : lc t),
-    CbvContraction (app (app elimUnit'' t) unit) (app t unit)
+    CbvContraction (elimUnit unit t) (app t unit)
 | CbvContraction_outl_pair :
   forall (v1 v2 : Tm)
     (Hv1 : CbvValue v1)
@@ -1450,92 +1143,34 @@ Inductive CbvContraction : Tm -> Tm -> Prop :=
     (Hv2 : CbvValue v2),
     CbvContraction (outr (pair v1 v2)) v2
 | CbvContraction_elimProd_pair :
-  forall (v1 v2 t : Tm) (l : list Atom)
-    (Hv1 : CbvValue v1)
-    (Hv2 : CbvValue v2)
-    (Hlc3 : forall x y : Atom, x # l -> y # x :: l -> lc (t {{ 0 ~> x }} {{ 1 ~> y }})),
-    CbvContraction (elimProd (pair v1 v2) t) (t {[ 0 ~> v1 ]} {[ 1 ~> v2 ]})
-| CbvContraction_elimProd'_pair :
   forall (v1 v2 t : Tm)
     (Hv1 : CbvValue v1)
     (Hv2 : CbvValue v2)
     (Hlc3 : lc t),
-    CbvContraction (elimProd' t (pair v1 v2)) (app (app t v1) v2)
-| CbvContraction_elimProd''_pair :
-  forall (v1 v2 t : Tm)
-    (Hv1 : CbvValue v1)
-    (Hv2 : CbvValue v2)
-    (Hlc3 : lc t),
-    CbvContraction (app (app elimProd'' t) (pair v1 v2)) (app (app t v1) v2)
+    CbvContraction (elimProd t (pair v1 v2)) (app (app t v1) v2)
 | CbvContraction_case_inl :
-  forall (t1 t2 t3 : Tm) (l : list Atom)
-    (Hv1 : CbvValue t1)
-    (Hlc2 : forall x : Atom, x # l -> lc (t2 {{ 0 ~> x }}))
-    (Hlc3 : forall x : Atom, x # l -> lc (t3 {{ 0 ~> x }})),
-    CbvContraction (case (inl t1) t2 t3) (t2 {[ 0 ~> t1 ]})
+  forall (t1 t2 t3 : Tm)
+    (Hlc1 : lc t1)
+    (Hlc2 : lc t2)
+    (Hv3 : CbvValue t3),
+    CbvContraction (case t1 t2 (inl t3)) (app t1 t3)
 | CbvContraction_case_inr :
-  forall (t1 t2 t3 : Tm) (l : list Atom)
-    (Hv1 : CbvValue t1)
-    (Hlc2 : forall x : Atom, x # l -> lc (t2 {{ 0 ~> x }}))
-    (Hlc3 : forall x : Atom, x # l -> lc (t3 {{ 0 ~> x }})),
-    CbvContraction (case (inr t1) t2 t3) (t3 {[ 0 ~> t1 ]})
-| CbvContraction_case'_inl :
   forall (t1 t2 t3 : Tm)
     (Hlc1 : lc t1)
     (Hlc2 : lc t2)
     (Hv3 : CbvValue t3),
-    CbvContraction (case' t1 t2 (inl t3)) (app t1 t3)
-| CbvContraction_case'_inr :
-  forall (t1 t2 t3 : Tm)
-    (Hlc1 : lc t1)
-    (Hlc2 : lc t2)
-    (Hv3 : CbvValue t3),
-    CbvContraction (case' t1 t2 (inr t3)) (app t2 t3)
-| CbvContraction_case''_inl :
-  forall (t1 t2 v : Tm)
-    (Hlc1 : lc t1)
-    (Hlc2 : lc t2)
-    (Hv : CbvValue v),
-    CbvContraction (app (app (app case'' t1) t2) (inl v)) (app t1 v)
-| CbvContraction_case''_inr :
-  forall (t1 t2 v : Tm)
-    (Hlc1 : lc t1)
-    (Hlc2 : lc t2)
-    (Hv : CbvValue v),
-    CbvContraction (app (app (app case'' t1) t2) (inr v)) (app t2 v)
+    CbvContraction (case t1 t2 (inr t3)) (app t2 t3)
 | CbvContraction_rec_zero :
-  forall (t1 t2 : Tm) (l : list Atom)
+  forall (t1 t2 : Tm)
     (Hlc1 : lc t1)
-    (Hlc2 : forall x : Atom, x # l -> lc (t2 {{ 0 ~> x }})),
+    (Hlc2 : lc t2),
     CbvContraction (rec t1 t2 zero) t1
 | CbvContraction_rec_succ :
-  forall (t1 t2 t3 : Tm) (l : list Atom)
-    (Hlc1 : lc t1)
-    (Hlc2 : forall x : Atom, x # l -> lc (t2 {{ 0 ~> x }}))
-    (Hv3 : CbvValue t3),
-    CbvContraction (rec t1 t2 (succ t3)) (t2 {[ 0 ~> rec t1 t2 t3 ]})
-| CbvContraction_rec'_zero :
-  forall (t1 t2 : Tm)
-    (Hlc1 : lc t1)
-    (Hlc2 : lc t2),
-    CbvContraction (rec' t1 t2 zero) t1
-| CbvContraction_rec'_succ :
   forall (t1 t2 t3 : Tm)
     (Hlc1 : lc t1)
     (Hlc2 : lc t2)
     (Hv3 : CbvValue t3),
-    CbvContraction (rec' t1 t2 (succ t3)) (app t2 (rec' t1 t2 t3))
-| CbvContraction_rec''_zero :
-  forall (t1 t2 : Tm)
-    (Hlc1 : lc t1)
-    (Hlc2 : lc t2),
-    CbvContraction (app (app (app rec'' t1) t2) zero) t1
-| CbvContraction_rec''_succ :
-  forall (t1 t2 t3 : Tm)
-    (Hlc1 : lc t1)
-    (Hlc2 : lc t2)
-    (Hv3 : CbvValue t3),
-    CbvContraction (app (app (app rec'' t1) t2) (succ t3)) (app t2 (app (app (app rec'' t1) t2) t3)).
+    CbvContraction (rec t1 t2 (succ t3)) (app t2 (rec t1 t2 t3)).
 
 #[export] Hint Constructors CbvContraction : core.
 
@@ -1543,14 +1178,14 @@ Lemma lc_CbvContraction_l :
   forall t t' : Tm,
     CbvContraction t t' -> lc t.
 Proof.
-  now inversion 1; subst; eauto 6.
+  now inversion 1; eauto.
 Qed.
 
 Lemma lc_CbvContraction_r :
   forall t t' : Tm,
     CbvContraction t t' -> lc t'.
 Proof.
-  now inversion 1; subst; eauto 6.
+  now inversion 1; eauto 6.
 Qed.
 
 #[export] Hint Immediate lc_CbvContraction_l lc_CbvContraction_r : core.
@@ -1592,20 +1227,10 @@ Inductive CbvAbortion : Tm -> Tm -> Prop :=
     (Hlc2 : lc t2),
     CbvAbortion (app (abort t1) t2) (abort t1)
 | CbvAbortion_elimUnit :
-  forall (t1 t2 : Tm) (l : list Atom)
+  forall (t1 t2 : Tm)
     (Hlc1 : lc t1)
-    (Hlc2 : forall x : Atom, x # l -> lc (t2 {{0 ~> x}})),
+    (Hlc2 : lc t2),
     CbvAbortion (elimUnit (abort t1) t2) (abort t1)
-| CbvAbortion_elimUnit' :
-  forall (t1 t2 : Tm)
-    (Hlc1 : lc t1)
-    (Hlc2 : lc t2),
-    CbvAbortion (elimUnit' (abort t1) t2) (abort t1)
-| CbvAbortion_elimUnit'' :
-  forall (t1 t2 : Tm)
-    (Hlc1 : lc t1)
-    (Hlc2 : lc t2),
-    CbvAbortion (app (app elimUnit'' t1) (abort t2)) (abort t2)
 | CbvAbortion_outl :
   forall (t : Tm)
     (Hlc' : lc  t),
@@ -1615,56 +1240,22 @@ Inductive CbvAbortion : Tm -> Tm -> Prop :=
     (Hlc' : lc  t),
     CbvAbortion (outr (abort t)) (abort t)
 | CbvAbortion_elimProd :
-  forall (t1 t2 : Tm) (l : list Atom)
-    (Hlc1 : lc t1)
-    (Hlc2 : forall x y : Atom, x # l -> y # x :: l -> lc (t2 {{ 0 ~> x }} {{ 1 ~> y }})),
-    CbvAbortion (elimProd (abort t1) t2) (abort t1)
-| CbvAbortion_elimProd' :
   forall (t1 t2 : Tm)
     (Hlc1 : lc t1)
     (Hlc2 : lc t2),
-    CbvAbortion (elimProd' t1 (abort t2)) (abort t2)
-| CbvAbortion_elimProd'' :
-  forall (t1 t2 : Tm)
-    (Hlc1 : lc t1)
-    (Hlc2 : lc t2),
-    CbvAbortion (app (app elimProd'' t1) (abort t2)) (abort t2)
+    CbvAbortion (elimProd t1 (abort t2)) (abort t2)
 | CbvAbortion_case :
-  forall (t1 t2 t3 : Tm) (l : list Atom)
-    (Hlc1 : lc t1)
-    (Hlc2 : forall x : Atom, x # l -> lc (t2 {{0 ~> x}}))
-    (Hlc3 : forall x : Atom, x # l -> lc (t3 {{0 ~> x}})),
-    CbvAbortion (case (abort t1) t2 t3) (abort t1)
-| CbvAbortion_case' :
   forall (t1 t2 t3 : Tm)
     (Hlc1 : lc t1)
     (Hlc2 : lc t2)
     (Hlc3 : lc t3),
-    CbvAbortion (case' t1 t2 (abort t3)) (abort t3)
-| CbvAbortion_case'' :
-  forall (t1 t2 t3 : Tm)
-    (Hlc1 : lc t1)
-    (Hlc2 : lc t2)
-    (Hlc3 : lc t3),
-    CbvAbortion (app (app (app case'' t1) t2) (abort t3)) (abort t3)
+    CbvAbortion (case t1 t2 (abort t3)) (abort t3)
 | CbvAbortion_rec :
-  forall (t1 t2 t3 : Tm) (l : list Atom)
-    (Hlc1 : lc t1)
-    (Hlc2 : forall x : Atom, x # l -> lc (t2 {{ 0 ~> x }}))
-    (Hlc3 : lc t3),
-    CbvAbortion (rec t1 t2 (abort t3)) (abort t3)
-| CbvAbortion_rec' :
   forall (t1 t2 t3 : Tm)
     (Hlc1 : lc t1)
     (Hlc2 : lc t2)
     (Hlc3 : lc t3),
-    CbvAbortion (rec' t1 t2 (abort t3)) (abort t3)
-| CbvAbortion_rec'' :
-  forall (t1 t2 t3 : Tm)
-    (Hlc1 : lc t1)
-    (Hlc2 : lc t2)
-    (Hlc3 : lc t3),
-    CbvAbortion (app (app (app rec'' t1) t2) (abort t3)) (abort t3).
+    CbvAbortion (rec t1 t2 (abort t3)) (abort t3).
 
 #[export] Hint Constructors CbvAbortion : core.
 
@@ -1742,20 +1333,10 @@ Inductive CbvStep : Tm -> Tm -> Prop :=
     CbvStep t2 t2' ->
     CbvStep (app (abs t1) t2) (app (abs t1) t2')
 | CbvStep_elimUnit :
-  forall (t1 t1' t2 : Tm) (l : list Atom)
-    (Hlc2 : forall x : Atom, x # l -> lc (t2 {{ 0 ~> x }})),
-    CbvStep t1 t1' ->
-    CbvStep (elimUnit t1 t2) (elimUnit t1' t2)
-| CbvStep_elimUnit' :
   forall (t1 t1' t2 : Tm)
     (Hlc2 : lc t2),
     CbvStep t1 t1' ->
-    CbvStep (elimUnit' t1 t2) (elimUnit' t1' t2)
-| CbvStep_elimUnit'' :
-  forall (t1 t2 t2' : Tm)
-    (Hlc1 : lc t1),
-    CbvStep t2 t2' ->
-    CbvStep (app (app elimUnit'' t1) t2) (app (app elimUnit'' t1) t2')
+    CbvStep (elimUnit t1 t2) (elimUnit t1' t2)
 | CbvStep_pair_l :
   forall (t1 t1' t2 : Tm),
     lc t2 ->
@@ -1775,20 +1356,10 @@ Inductive CbvStep : Tm -> Tm -> Prop :=
     CbvStep t t' ->
     CbvStep (outr t) (outr t')
 | CbvStep_elimProd :
-  forall (t1 t1' t2 : Tm) (l : list Atom)
-    (Hs1 : CbvStep t1 t1')
-    (Hlc2 : forall x y : Atom, x # l -> y # x :: l -> lc (t2 {{ 0 ~> x }} {{ 1 ~> y }})),
-    CbvStep (elimProd t1 t2) (elimProd t1' t2)
-| CbvStep_elimProd' :
   forall (t1 t2 t2' : Tm)
     (Hlc1 : lc t1)
     (Hs2 : CbvStep t2 t2'),
-    CbvStep (elimProd' t1 t2) (elimProd' t1 t2')
-| CbvStep_elimProd'' :
-  forall (t1 t2 t2' : Tm)
-    (Hlc1 : lc t1)
-    (Hs2 : CbvStep t2 t2'),
-    CbvStep (app (app elimProd'' t1) t2) (app (app elimProd'' t1) t2')
+    CbvStep (elimProd t1 t2) (elimProd t1 t2')
 | CbvStep_inl :
   forall t t' : Tm,
     CbvStep t t' ->
@@ -1798,45 +1369,21 @@ Inductive CbvStep : Tm -> Tm -> Prop :=
     CbvStep t t' ->
     CbvStep (inr t) (inr t')
 | CbvStep_case :
-  forall (t1 t1' t2 t3 : Tm) (l : list Atom)
-    (Hlc2 : forall x : Atom, x # l -> lc (t2 {{ 0 ~> x }}))
-    (Hlc3 : forall x : Atom, x # l -> lc (t3 {{ 0 ~> x }})),
-    CbvStep t1 t1' ->
-    CbvStep (case t1 t2 t3) (case t1' t2 t3)
-| CbvStep_case' :
   forall (t1 t2 t3 t3' : Tm)
     (Hlc1 : lc t1)
     (Hlc2 : lc t2)
     (Hs3 : CbvStep t3 t3'),
-    CbvStep (case' t1 t2 t3) (case' t1 t2 t3')
-| CbvStep_case'' :
-  forall (t1 t2 t3 t3' : Tm)
-    (Hlc1 : lc t1)
-    (Hlc2 : lc t2)
-    (Hs3 : CbvStep t3 t3'),
-    CbvStep (app (app (app case'' t1) t2) t3) (app (app (app case'' t1) t2) t3')
+    CbvStep (case t1 t2 t3) (case t1 t2 t3')
 | CbvStep_succ :
   forall (t t' : Tm),
     CbvStep t t' ->
     CbvStep (succ t) (succ t')
 | CbvStep_rec :
-  forall (t1 t2 t3 t3' : Tm) (l : list Atom)
-    (Hlc1 : lc t1)
-    (Hlc2 : forall x : Atom, x # l -> lc (t2 {{ 0 ~> x }}))
-    (Hs3 : CbvStep t3 t3'),
-    CbvStep (rec t1 t2 t3) (rec t1 t2 t3')
-| CbvStep_rec' :
   forall (t1 t2 t3 t3' : Tm)
     (Hlc1 : lc t1)
     (Hlc2 : lc t2)
     (Hs3 : CbvStep t3 t3'),
-    CbvStep (rec' t1 t2 t3) (rec' t1 t2 t3')
-| CbvStep_rec'' :
-  forall (t1 t2 t3 t3' : Tm)
-    (Hlc1 : lc t1)
-    (Hlc2 : lc t2)
-    (Hs3 : CbvStep t3 t3'),
-    CbvStep (app (app (app rec'' t1) t2) t3) (app (app (app rec'' t1) t2) t3').
+    CbvStep (rec t1 t2 t3) (rec t1 t2 t3').
 
 #[export] Hint Constructors CbvStep : core.
 
@@ -1933,72 +1480,13 @@ Lemma progress_cbv :
 Proof.
   intros t A Ht.
   remember [] as Γ.
-  induction Ht; subst; try now auto. Focus 2.
-    repeat match goal with
-    | Ht : Typing _ ?t _, IH : [] = [] -> CbvValue ?t \/ _ |- _ =>
-      destruct (IH eq_refl) as [ | [] ]; [| now eauto 6]; clear IH
-    end.
-
-  try match goal with
-  | Hv : CbvValue ?t, Ht : Typing _ ?t _ |- _ =>
-    inversion Hv; subst; clear Hv;
-    inversion Ht; subst; clear Ht
-  end;
-
-  repeat (match goal with
-  | Ht : Typing _ ?t _ |- _ =>
-    tryif is_var t then fail else inversion Ht; subst; clear Ht
-  end).
-
-
-
-(*
-  destruct (IHHt1 eq_refl) as [ Hv1 | [t1' Hs1] ]; [| now eauto].
-  destruct (IHHt2 eq_refl) as [ Hv2 | [t2' Hs2] ]; [| now eauto].
-  Time inversion Hv1; subst;
-    repeat (auto; match goal with
-    | H : Typing _ (const _) _ |- _ => inversion H; subst; clear H
-    | H : Typing _ (app _ _) _ |- _ => inversion H; subst; clear H
-    end); eauto 7;
-  match goal with
-  | |- context [CbvValue (app _ ?t)] =>
-    repeat match goal with
-    | Hv : CbvValue t, Ht : Typing [] t _ |- _ =>
-      inversion Hv; subst; inversion Ht; subst
-    | H : Typing _ (const _) _ |- _ => inversion H; subst; clear H
-    | H : Typing _ (app _ _) _ |- _ => inversion H; subst; clear H
-    end
-  end; eauto 8.
-*)
-Restart.
-  intros t A Ht.
-  remember [] as Γ.
   induction Ht; subst; try now auto.
   - now left; eauto.
   - destruct (IHHt1 eq_refl) as [ Hv | [t1' Hs1] ]; [| now eauto].
-    inversion Hv; subst; inversion Ht1; subst; only 2, 4-5, 7-8: now eauto 6.
+    inversion Hv; subst; inversion Ht1; subst; try now auto.
     + now destruct (IHHt2 eq_refl) as [ Hv2 | [t2' Hs2] ]; eauto.
-    + destruct (IHHt2 eq_refl) as [ Hv2 | [t2' Hs2] ]; [| now eauto].
-      inversion Ht0; subst.
-      inversion Ht2; subst; inversion Hv2; subst; try now eauto.
-      * now inversion Ht4; inversion Ht6.
-      * now inversion Ht4; inversion Ht6.
-    + destruct (IHHt2 eq_refl) as [ Hv2 | [t2' Hs2] ]; [| now eauto].
-      inversion Ht0; subst.
-      inversion Ht2; subst; inversion Hv2; subst; try now eauto.
-      * now inversion Ht4; inversion Ht6.
-      * now inversion Ht4; inversion Ht6.
-    + destruct (IHHt2 eq_refl) as [ Hv2 | [t2' Hs2] ]; [| now eauto].
-      inversion Ht0; inversion Ht4; subst.
-      inversion Ht2; subst; inversion Hv2; subst; try now eauto.
-      * now inversion Ht2; subst; inversion Ht6; subst; inversion Ht10.
-      * now inversion Ht2; subst; inversion Ht6; subst; inversion Ht10.
-    + now destruct (IHHt2 eq_refl) as [ Hv2 | [t2' Hs2] ]; eauto.
-    + destruct (IHHt2 eq_refl) as [ Hv2 | [t2' Hs2] ]; [| now eauto].
-      now inversion Ht0; inversion Ht4; subst.
+    + now eauto 6.
   - now right; eauto.
-  - right; destruct (IHHt eq_refl) as [Hv | [t'' Hs] ]; [| now eauto].
-    now inversion Hv; subst; inversion Ht; subst; try (now inversion Ht1); eauto 6.
   - right; destruct (IHHt1 eq_refl) as [ Hv | [t1' Hs1] ]; [| now eauto].
     now inversion Hv; subst; inversion Ht1; subst; try (now inversion Ht0); eauto 6.
   - now left; eauto.
@@ -2007,21 +1495,13 @@ Restart.
     now inversion Hv; subst; inversion Ht; subst; try (now inversion Ht1); eauto 6.
   - right; destruct (IHHt eq_refl) as [Hv | [t'' Hs] ]; [| now eauto].
     now inversion Hv; subst; inversion Ht; subst; try (now inversion Ht1); eauto 6.
-  - right; destruct (IHHt eq_refl) as [Hv | [t'' Hs] ]; [| now eauto 6].
-    now inversion Hv; subst; inversion Ht; subst; try (now inversion Ht1); eauto 6.
   - right; destruct (IHHt2 eq_refl) as [Hv | [t'' Hs] ]; [| now eauto 6].
     now inversion Hv; subst; inversion Ht2; subst; try (now inversion Ht0); eauto 6.
   - now destruct (IHHt eq_refl) as [Hv | [t'' Hs] ]; eauto.
   - now destruct (IHHt eq_refl) as [Hv | [t'' Hs] ]; eauto.
-  - right; destruct (IHHt eq_refl) as [Hv | [t'' Hs] ].
-    + now inversion Hv; subst; inversion Ht; subst; try (now inversion Ht1);
-        eexists; do 2 econstructor; unshelve eauto.
-    + now eexists; econstructor; unshelve eauto.
   - right; destruct (IHHt3 eq_refl) as [Hv3 | [] ]; [| now eauto].
     now inversion Hv3; subst; inversion Ht3; subst; try (now inversion Ht0); eauto 6.
   - now destruct (IHHt eq_refl) as [Hv | [t'' Hs] ]; eauto.
-  - right; destruct (IHHt2 eq_refl) as [Hv1 | [t1' Hs1] ]; [| now eauto 6].
-    now inversion Hv1; subst; inversion Ht3; subst; try (now inversion Ht0); eauto 7.
   - right; destruct (IHHt3 eq_refl) as [Hv1 | [t1' Hs1] ]; [| now eauto 6].
     now inversion Hv1; subst; inversion Ht3; subst; try (now inversion Ht0); eauto 7.
 Qed.
@@ -2036,11 +1516,6 @@ Inductive CbnValue : Tm -> Prop :=
     (Hlc' : forall x : Atom, x # l -> lc (t' {{ 0 ~> x }})),
     CbnValue (abs t')
 | CbnValue_unit : CbnValue unit
-| CbnValue_elimUnit'' : CbnValue elimUnit''
-| CbnValue_elimUnit''1 :
-  forall (t' : Tm)
-    (Hlc' : lc t'),
-    CbnValue (app elimUnit'' t')
 | CbnValue_abort :
   forall (t' : Tm)
     (Hlc' : lc t'),
@@ -2050,11 +1525,6 @@ Inductive CbnValue : Tm -> Prop :=
     (Hlc1 : lc t1)
     (Hlc2 : lc t2),
     CbnValue (pair t1 t2)
-| CbnValue_elimProd'' : CbnValue elimProd''
-| CbnValue_elimProd''1 :
-  forall (t1 : Tm)
-    (Hlc1 : lc t1),
-    CbnValue (app elimProd'' t1)
 | CbnValue_inl :
   forall (t' : Tm)
     (Hlc' : lc t'),
@@ -2063,31 +1533,11 @@ Inductive CbnValue : Tm -> Prop :=
   forall (t' : Tm)
     (Hlc' : lc t'),
     CbnValue (inr t')
-| CbnValue_case'' : CbnValue case''
-| CbnValue_case''1 :
-  forall (t1 : Tm)
-    (Hlc1 : lc t1),
-    CbnValue (app case'' t1)
-| CbnValue_case''2 :
-  forall (t1 t2 : Tm)
-    (Hlc1 : lc t1)
-    (Hlc2 : lc t2),
-    CbnValue (app (app case'' t1) t2)
 | CbnValue_zero : CbnValue zero
 | CbnValue_succ :
   forall (t' : Tm)
     (Hlc' : lc t'),
-    CbnValue (succ t')
-| CbnValue_rec'' : CbnValue rec''
-| CbnValue_rec''1 :
-  forall (t1 : Tm)
-    (Hlc1 : lc t1),
-    CbnValue (app rec'' t1)
-| CbnValue_rec''2 :
-  forall (t1 t2 : Tm)
-    (Hlc1 : lc t1)
-    (Hlc2 : lc t2),
-    CbnValue (app (app rec'' t1) t2).
+    CbnValue (succ t').
 
 #[export] Hint Constructors CbnValue : core.
 
@@ -2113,20 +1563,10 @@ Inductive CbnContraction : Tm -> Tm -> Prop :=
     (Hlc : lc t),
     CbnContraction (annot t A) t
 | CbnContraction_elimUnit :
-  forall (t1 t2 : Tm) (l : list Atom)
-    (Hlc1 : lc t1)
-    (Hlc2 : forall x : Atom, x # l -> lc (t2 {{0 ~> x}})),
-    CbnContraction (elimUnit t1 t2) (t2 {[ 0 ~> unit ]})
-| CbnContraction_elimUnit' :
   forall (t1 t2 : Tm)
     (Hlc1 : lc t1)
     (Hlc2 : lc t2),
-    CbnContraction (elimUnit' t1 t2) (app t2 unit)
-| CnvContraction_app_elimUnit'' :
-  forall (t1 t2 : Tm)
-    (Hlc1 : lc t1)
-    (Hlc2 : lc t2),
-    CbnContraction (app (app elimUnit'' t1) t2) (app t1 unit)
+    CbnContraction (elimUnit t1 t2) (app t2 unit)
 | CbnContraction_outl_pair :
   forall (t1 t2 : Tm)
     (Hlc1 : lc t1)
@@ -2138,92 +1578,34 @@ Inductive CbnContraction : Tm -> Tm -> Prop :=
     (Hlc2 : lc t2),
     CbnContraction (outr (pair t1 t2)) t2
 | CbnContraction_elimProd_pair :
-  forall (t1 t2 t3 : Tm) (l : list Atom)
-    (Hlc1 : lc t1)
-    (Hlc2 : lc t2)
-    (Hlc3 : forall x y : Atom, x # l -> y # x :: l -> lc (t3 {{ 0 ~> x }} {{ 1 ~> y }})),
-    CbnContraction (elimProd (pair t1 t2) t3) (t3 {[ 0 ~> t1 ]} {[ 1 ~> t2 ]})
-| CbnContraction_elimProd'_pair :
   forall (t1 t2 t3 : Tm)
     (Hlc1 : lc t1)
     (Hlc2 : lc t2)
     (Hlc3 : lc t3),
-    CbnContraction (elimProd' t1 (pair t2 t3)) (app (app t1 t2) t3)
-| CbnContraction_elimProd''_pair :
-  forall (t1 t2 t3 : Tm)
-    (Hlc1 : lc t1)
-    (Hlc2 : lc t2)
-    (Hlc3 : lc t3),
-    CbnContraction (app (app elimProd'' t1) (pair t2 t3)) (app (app t1 t2) t3)
+    CbnContraction (elimProd t1 (pair t2 t3)) (app (app t1 t2) t3)
 | CbnContraction_case_inl :
-  forall (t1 t2 t3 : Tm) (l : list Atom)
+  forall (t1 t2 t3 : Tm)
     (Hlc1 : lc t1)
-    (Hlc2 : forall x : Atom, x # l -> lc (t2 {{ 0 ~> x }}))
-    (Hlc3 : forall x : Atom, x # l -> lc (t3 {{ 0 ~> x }})),
-    CbnContraction (case (inl t1) t2 t3) (t2 {[ 0 ~> t1 ]})
+    (Hlc2 : lc t2)
+    (Hlc3 : lc t3),
+    CbnContraction (case t1 t2 (inl t3)) (app t1 t3)
 | CbnContraction_case_inr :
-  forall (t1 t2 t3 : Tm) (l : list Atom)
-    (Hlc1 : lc t1)
-    (Hlc2 : forall x : Atom, x # l -> lc (t2 {{ 0 ~> x }}))
-    (Hlc3 : forall x : Atom, x # l -> lc (t3 {{ 0 ~> x }})),
-    CbnContraction (case (inr t1) t2 t3) (t3 {[ 0 ~> t1 ]})
-| CbnContraction_case'_inl :
   forall (t1 t2 t3 : Tm)
     (Hlc1 : lc t1)
     (Hlc2 : lc t2)
     (Hlc3 : lc t3),
-    CbnContraction (case' t1 t2 (inl t3)) (app t1 t3)
-| CbnContraction_case'_inr :
-  forall (t1 t2 t3 : Tm)
-    (Hlc1 : lc t1)
-    (Hlc2 : lc t2)
-    (Hlc3 : lc t3),
-    CbnContraction (case' t1 t2 (inr t3)) (app t2 t3)
-| CbnContraction_case''_inl :
-  forall (t1 t2 t3 : Tm)
-    (Hlc1 : lc t1)
-    (Hlc2 : lc t2)
-    (Hlc3 : lc t3),
-    CbnContraction (app (app (app case'' t1) t2) (inl t3)) (app t1 t3)
-| CbnContraction_case''_inr :
-  forall (t1 t2 t3 : Tm)
-    (Hlc1 : lc t1)
-    (Hlc2 : lc t2)
-    (Hlc3 : lc t3),
-    CbnContraction (app (app (app case'' t1) t2) (inr t3)) (app t2 t3)
+    CbnContraction (case t1 t2 (inr t3)) (app t2 t3)
 | CbnContraction_rec_zero :
-  forall (t1 t2 : Tm) (l : list Atom)
+  forall (t1 t2 : Tm)
     (Hlc1 : lc t1)
-    (Hlc2 : forall x : Atom, x # l -> lc (t2 {{ 0 ~> x }})),
+    (Hlc2 : lc t2),
     CbnContraction (rec t1 t2 zero) t1
 | CbnContraction_rec_succ :
-  forall (t1 t2 t3 : Tm) (l : list Atom)
-    (Hlc1 : lc t1)
-    (Hlc2 : forall x : Atom, x # l -> lc (t2 {{ 0 ~> x }}))
-    (Hlc3 : lc t3),
-    CbnContraction (rec t1 t2 (succ t3)) (t2 {[ 0 ~> rec t1 t2 t3 ]})
-| CbnContraction_rec'_zero :
-  forall (t1 t2 : Tm)
-    (Hlc1 : lc t1)
-    (Hlc2 : lc t2),
-    CbnContraction (rec' t1 t2 zero) t1
-| CbnContraction_rec'_succ :
   forall (t1 t2 t3 : Tm)
     (Hlc1 : lc t1)
     (Hlc2 : lc t2)
     (Hlc3 : lc t3),
-    CbnContraction (rec' t1 t2 (succ t3)) (app t2 (rec' t1 t2 t3))
-| CbnContraction_rec''_zero :
-  forall (t1 t2 : Tm)
-    (Hlc1 : lc t1)
-    (Hlc2 : lc t2),
-    CbnContraction (app (app (app rec'' t1) t2) zero) t1
-| CbnContraction_rec''_succ :
-  forall (t1 t2 t3 : Tm)
-    (Hlc1 : lc t1)
-    (Hlc2 : lc t2)
-    (Hlc3 : lc t3),
-    CbnContraction (app (app (app rec'' t1) t2) (succ t3)) (app t2 (app (app (app rec'' t1) t2) t3)).
+    CbnContraction (rec t1 t2 (succ t3)) (app t2 (rec t1 t2 t3)).
 
 #[export] Hint Constructors CbnContraction : core.
 
@@ -2288,56 +1670,22 @@ Inductive CbnAbortion : Tm -> Tm -> Prop :=
     (Hlc' : lc  t),
     CbnAbortion (outr (abort t)) (abort t)
 | CbnAbortion_elimProd :
-  forall (t1 t2 : Tm) (l : list Atom)
-    (Hlc1 : lc t1)
-    (Hlc2 : forall x y : Atom, x # l -> y # x :: l -> lc (t2 {{ 0 ~> x }} {{ 1 ~> y }})),
-    CbnAbortion (elimProd (abort t1) t2) (abort t1)
-| CbnAbortion_elimProd' :
   forall (t1 t2 : Tm)
     (Hlc1 : lc t1)
     (Hlc2 : lc t2),
-    CbnAbortion (elimProd' t1 (abort t2)) (abort t2)
-| CbnAbortion_elimProd'' :
-  forall (t1 t2 : Tm)
-    (Hlc1 : lc t1)
-    (Hlc2 : lc t2),
-    CbnAbortion (app (app elimProd'' t1) (abort t2)) (abort t2)
+    CbnAbortion (elimProd t1 (abort t2)) (abort t2)
 | CbnAbortion_case :
-  forall (t1 t2 t3 : Tm) (l : list Atom)
-    (Hlc1 : lc t1)
-    (Hlc2 : forall x : Atom, x # l -> lc (t2 {{0 ~> x}}))
-    (Hlc3 : forall x : Atom, x # l -> lc (t3 {{0 ~> x}})),
-    CbnAbortion (case (abort t1) t2 t3) (abort t1)
-| CbnAbortion_case' :
   forall (t1 t2 t3 : Tm)
     (Hlc1 : lc t1)
     (Hlc2 : lc t2)
     (Hlc3 : lc t3),
-    CbnAbortion (case' t1 t2 (abort t3)) (abort t3)
-| CbnAbortion_case'' :
-  forall (t1 t2 t3 : Tm)
-    (Hlc1 : lc t1)
-    (Hlc2 : lc t2)
-    (Hlc3 : lc t3),
-    CbnAbortion (app (app (app case'' t1) t2) (abort t3)) (abort t3)
+    CbnAbortion (case t1 t2 (abort t3)) (abort t3)
 | CbnAbortion_rec :
-  forall (t1 t2 t3 : Tm) (l : list Atom)
-    (Hlc1 : lc t1)
-    (Hlc2 : forall x : Atom, x # l -> lc (t2 {{ 0 ~> x }}))
-    (Hlc3 : lc t3),
-    CbnAbortion (rec t1 t2 (abort t3)) (abort t3)
-| CbnAbortion_rec' :
   forall (t1 t2 t3 : Tm)
     (Hlc1 : lc t1)
     (Hlc2 : lc t2)
     (Hlc3 : lc t3),
-    CbnAbortion (rec' t1 t2 (abort t3)) (abort t3)
-| CbnAbortion_rec'' :
-  forall (t1 t2 t3 : Tm)
-    (Hlc1 : lc t1)
-    (Hlc2 : lc t2)
-    (Hlc3 : lc t3),
-    CbnAbortion (app (app (app rec'' t1) t2) (abort t3)) (abort t3).
+    CbnAbortion (rec t1 t2 (abort t3)) (abort t3).
 
 #[export] Hint Constructors CbnAbortion : core.
 
@@ -2418,56 +1766,22 @@ Inductive CbnStep : Tm -> Tm -> Prop :=
     CbnStep t t' ->
     CbnStep (outr t) (outr t')
 | CbnStep_elimProd :
-  forall (t1 t1' t2 : Tm) (l : list Atom)
-    (Hs1 : CbnStep t1 t1')
-    (Hlc2 : forall x y : Atom, x # l -> y # x :: l -> lc (t2 {{ 0 ~> x }} {{ 1 ~> y }})),
-    CbnStep (elimProd t1 t2) (elimProd t1' t2)
-| CbnStep_elimProd' :
   forall (t1 t2 t2' : Tm)
     (Hlc1 : lc t1)
     (Hs2 : CbnStep t2 t2'),
-    CbnStep (elimProd' t1 t2) (elimProd' t1 t2')
-| CbnStep_elimProd'' :
-  forall (t1 t2 t2' : Tm)
-    (Hlc1 : lc t1)
-    (Hs2 : CbnStep t2 t2'),
-    CbnStep (app (app elimProd'' t1) t2) (app (app elimProd'' t1) t2')
+    CbnStep (elimProd t1 t2) (elimProd t1 t2')
 | CbnStep_case :
-  forall (t1 t1' t2 t3 : Tm) (l : list Atom)
-    (Hlc2 : forall x : Atom, x # l -> lc (t2 {{ 0 ~> x }}))
-    (Hlc3 : forall x : Atom, x # l -> lc (t3 {{ 0 ~> x }})),
-    CbnStep t1 t1' ->
-    CbnStep (case t1 t2 t3) (case t1' t2 t3)
-| CbnStep_case' :
   forall (t1 t2 t3 t3' : Tm)
     (Hlc1 : lc t1)
     (Hlc2 : lc t2)
     (Hs3 : CbnStep t3 t3'),
-    CbnStep (case' t1 t2 t3) (case' t1 t2 t3')
-| CbnStep_case'' :
-  forall (t1 t2 t3 t3' : Tm)
-    (Hlc1 : lc t1)
-    (Hlc2 : lc t2)
-    (Hs3 : CbnStep t3 t3'),
-    CbnStep (app (app (app case'' t1) t2) t3) (app (app (app case'' t1) t2) t3')
+    CbnStep (case t1 t2 t3) (case t1 t2 t3')
 | CbnStep_rec :
-  forall (t1 t2 t3 t3' : Tm) (l : list Atom)
-    (Hlc1 : lc t1)
-    (Hlc2 : forall x : Atom, x # l -> lc (t2 {{ 0 ~> x }}))
-    (Hs3 : CbnStep t3 t3'),
-    CbnStep (rec t1 t2 t3) (rec t1 t2 t3')
-| CbnStep_rec' :
   forall (t1 t2 t3 t3' : Tm)
     (Hlc1 : lc t1)
     (Hlc2 : lc t2)
     (Hs3 : CbnStep t3 t3'),
-    CbnStep (rec' t1 t2 t3) (rec' t1 t2 t3')
-| CbnStep_rec'' :
-  forall (t1 t2 t3 t3' : Tm)
-    (Hlc1 : lc t1)
-    (Hlc2 : lc t2)
-    (Hs3 : CbnStep t3 t3'),
-    CbnStep (app (app (app rec'' t1) t2) t3) (app (app (app rec'' t1) t2) t3').
+    CbnStep (rec t1 t2 t3) (rec t1 t2 t3').
 
 #[export] Hint Constructors CbnStep : core.
 
@@ -2563,52 +1877,36 @@ Lemma progress_cbn :
 Proof.
   intros t A Ht.
   remember [] as Γ.
-  induction Ht; subst.
-  - now inversion Hwf.
+  induction Ht; subst; try now auto.
   - now left; eauto.
   - destruct (IHHt1 eq_refl) as [ Hv | [t1' Hs1] ]; [| now eauto].
-    inversion Hv; subst; inversion Ht1; subst; only 1-5, 7-8, 10: now eauto 6.
-    + destruct (IHHt2 eq_refl) as [ Hv2 | [t2' Hs2] ]; [| now eauto].
-      inversion Ht0; subst.
-      inversion Ht2; subst; inversion Hv2; subst; try now eauto.
-      * now inversion Ht4; inversion Ht6.
-      * now inversion Ht4; inversion Ht6.
-    + destruct (IHHt2 eq_refl) as [ Hv2 | [t2' Hs2] ]; [| now eauto].
-      inversion Ht0; inversion Ht4; subst.
-      inversion Ht2; subst; inversion Hv2; subst; try now eauto.
-      * inversion Ht2; subst; inversion Ht6; subst; inversion Ht10.
-      * inversion Ht2; subst; inversion Ht6; subst; inversion Ht10.
-    + destruct (IHHt2 eq_refl) as [ Hv2 | [t2' Hs2] ]; [| now eauto].
-      now inversion Ht0; inversion Ht4; subst.
+    now inversion Hv; subst; inversion Ht1; subst; eauto 6.
   - now right; eauto.
-  - now left.
-  - now right; eauto 7.
-  - now right; eauto 7.
-  - now left.
+  - right; destruct (IHHt1 eq_refl) as [ Hv | [t1' Hs1] ]; [| now eauto 6].
+    now inversion Hv; subst; inversion Ht1; subst; try (now inversion Ht0); eauto 6.
   - now left; eauto.
   - now destruct (IHHt1 eq_refl) as [| [] ], (IHHt2 eq_refl) as [| [] ]; eauto.
   - right; destruct (IHHt eq_refl) as [Hv | [t'' Hs] ]; [| now eauto].
     now inversion Hv; subst; inversion Ht; subst; try (now inversion Ht1); eauto 6.
   - right; destruct (IHHt eq_refl) as [Hv | [t'' Hs] ]; [| now eauto].
     now inversion Hv; subst; inversion Ht; subst; try (now inversion Ht1); eauto 6.
-  - right; destruct (IHHt eq_refl) as [Hv | [t'' Hs] ]; [| now eauto 6].
-    now inversion Hv; subst; inversion Ht; subst; try (now inversion Ht1); eauto 6.
   - right; destruct (IHHt2 eq_refl) as [Hv | [t'' Hs] ]; [| now eauto 6].
     now inversion Hv; subst; inversion Ht2; subst; try (now inversion Ht0); eauto 6.
-  - now left.
   - now destruct (IHHt eq_refl) as [Hv | [t'' Hs] ]; eauto.
   - now destruct (IHHt eq_refl) as [Hv | [t'' Hs] ]; eauto.
-  - right; destruct (IHHt eq_refl) as [Hv | [t'' Hs] ].
-    + now inversion Hv; subst; inversion Ht; subst; try (now inversion Ht1);
-        eexists; do 2 econstructor; intros; try eapply lc_Typing; eauto.
-    + now eexists; econstructor; intros; try eapply lc_Typing; eauto.
   - right; destruct (IHHt3 eq_refl) as [Hv3 | [] ]; [| now eauto].
     now inversion Hv3; subst; inversion Ht3; subst; try (now inversion Ht0); eauto 6.
-  - now left.
-  - now left.
   - now destruct (IHHt eq_refl) as [Hv | [t'' Hs] ]; eauto.
-  - right; destruct (IHHt2 eq_refl) as [Hv1 | [t1' Hs1] ]; [| now eauto 6].
-    now inversion Hv1; subst; inversion Ht3; subst; try (now inversion Ht0); eauto 7.
   - right; destruct (IHHt3 eq_refl) as [Hv1 | [t1' Hs1] ]; [| now eauto 6].
     now inversion Hv1; subst; inversion Ht3; subst; try (now inversion Ht0); eauto 7.
 Qed.
+
+Lemma Cbv_Cbn :
+  forall (t1 t2 : Tm),
+    CbvAbortion t1 t2 <-> CbnAbortion t1 t2.
+Proof.
+  split.
+  - inversion 1; eauto.
+    admit.
+  - inversion 1; eauto.
+Admitted.
